src/Helpers.dfy
@@ -5,31 +5,10 @@
 *  SPDX-License-Identifier: MIT 
 *******************************************************************************/
 
-include "Wrappers.dfy"
-include "UInt.dfy"
-include "Relations.dfy"
-
 module Helpers {
   export 
     provides Comparison
 
-  import opened Comparison
-  import opened U = UInt
-  import Relations
-  import opened Wrappers
-
-
-  /*
-   * Here is an example relation and a lemma that says the relation is appropriate for use in
-   * lexicographic orderings.
-   */
-
-  lemma UInt8LessIsTrichotomousTransitive()
-    ensures Relations.Trichotomous(UInt8Less)
-    ensures Relations.Transitive(UInt8Less)
-  {
-  }
-  
 }
 
 module Helpers.Comparison {
